src/Parsers/ContextFreeGrammar/Fix/FromAbstractInterpretation.v
@@ -9,6 +9,7 @@ Require Import Fiat.Parsers.ContextFreeGrammar.Fix.FromAbstractInterpretationDef
 Require Import Fiat.Parsers.ContextFreeGrammar.Fix.Fix.
 Require Import Fiat.Parsers.ContextFreeGrammar.Fix.Definitions.
 Require Import Fiat.Parsers.ContextFreeGrammar.Fix.Correct.
+Require Import Fiat.Common.BoolFacts.
 
 Set Implicit Arguments.
 Local Coercion is_true : bool >-> Sortclass.
@@ -16,129 +17,151 @@ Local Open Scope list_scope.
 Local Open Scope grammar_fixedpoint_scope.
 
 Section fold_correctness.
-  Context {Char : Type} {HSLM : StringLikeMin Char} {HSL : StringLike Char}
-          {irdata : Reflective.interp_RCharExpr_data Char}.
+  Context {Char : Type} {HSLM : StringLikeMin Char} {HSL : StringLike Char}.
   Context {T : Type}.
   Context {fpdata : @grammar_fixedpoint_lattice_data T}
           {aidata : @AbstractInterpretation Char T}
           (related : Ensemble String -> T -> Prop)
           {aicdata : AbstractInterpretationCorrectness related}.
-  Context (G : pregrammar Char).
+  Context (G : pregrammar' Char).
 
   Let predata := @rdp_list_predata _ G.
   Local Existing Instance predata.
 
   Definition fold_grammar : aggregate_state (fixedpoint_by_abstract_interpretation G)
-    := pre_Fix_grammar _ G.
+    := pre_Fix_grammar _ initial_nonterminals_data.
+
+  Record ensemble_result (str : String) (fold_state : T) :=
+    { er_ensemble :> Ensemble String;
+      er_state :> T;
+      er_related :> related er_ensemble er_state;
+      er_correct :> Ensembles.In _ er_ensemble str;
+      er_state_le :> fold_state <= er_state }.
+
+  Definition er_lift {str st1 st2}
+             (v : ensemble_result str st1)
+             (Hle : st2 <= st1)
+    : ensemble_result str st2
+    := {| er_ensemble := v;
+          er_state := v;
+          er_related := er_related v;
+          er_correct := er_correct v;
+          er_state_le := transitivity Hle (er_state_le v) |}.
+
+  Definition er_combine_production n str st1 st2 (it : ensemble_result (take n str) st1) (its : ensemble_result (drop n str) st2)
+    : ensemble_result str (combine_production st1 st2)
+    := {| er_ensemble := ensemble_combine_production it its;
+          er_state := combine_production (T := T) it its;
+          er_related := combine_production_correct (er_related it) (er_related its);
+          er_correct := ex_intro _ n (conj (er_correct it) (er_correct its));
+          er_state_le := combine_production_Proper_le (er_state_le it) (er_state_le its) |}.
+
+  Lemma fold_le nt st
+        (H : fold_productions' G (lookup_state fold_grammar) (Lookup_string G nt) <= st)
+    : lookup_state fold_grammar (of_nonterminal nt) <= st.
+  Proof.
+    unfold fold_grammar.
+    rewrite pre_Fix_grammar_fixedpoint.
+    unfold aggregate_step.
+    rewrite lookup_state_aggregate_state_glb, greatest_lower_bound_correct_r.
+    rewrite lookup_state_aggregate_prestep, (find_pre_Fix_grammar_to_lookup_state _ G).
+    let v := match goal with |- context[if ?v then _ else _] => v end in
+    destruct v eqn:Hvalid; unfold option_rect; [ | apply bottom_bottom ].
+    unfold step_constraints.
+    unfold fixedpoint_by_abstract_interpretation at 1.
+    unfold fold_constraints.
+    rewrite <- list_to_productions_to_nonterminal.
+    change (default_to_nonterminal ?nt) with (to_nonterminal nt).
+    rewrite to_of_nonterminal by (eapply initial_nonterminals_correct; assumption).
+    assumption.
+  Qed.
+
+  Definition lift_ensemble_result {str nt}
+             (res : ensemble_result str (fold_productions' G (lookup_state fold_grammar) (G nt)))
+    : ensemble_result str (lookup_state fold_grammar (of_nonterminal nt))
+    := {| er_ensemble := er_ensemble res;
+          er_state := er_state res;
+          er_related := er_related res;
+          er_correct := er_correct res;
+          er_state_le := fold_le _ _ (er_state_le res) |}.
 
   Section step.
-    Context (state_of_parse : forall str pats, parse_of G str pats -> T)
-            (state_of_parse_production : forall str pat, parse_of_production G str pat -> T)
-            (state_of_parse_item : forall str it, parse_of_item G str it -> T).
+    Context (state_of_parse : forall str pats, parse_of G str pats -> ensemble_result str (fold_productions' G (lookup_state fold_grammar) pats))
+            (state_of_parse_production : forall str pat, parse_of_production G str pat -> ensemble_result str (fold_production' G (lookup_state fold_grammar) pat))
+            (state_of_parse_item : forall str it, parse_of_item G str it -> ensemble_result str (fold_item' G (lookup_state fold_grammar) it)).
 
     Definition state_of_parse_item'
                str it (p : parse_of_item G str it)
-      : T
-      := match p with
-         | ParseTerminal ch P Hch Hstr => on_terminal P
-         | ParseNonTerminal nt Hvalid p' => state_of_parse p'
+      : ensemble_result str (fold_item' G (lookup_state fold_grammar) it)
+      := match p in parse_of_item _ _ it return ensemble_result _ (fold_item' _ _ it) with
+         | ParseTerminal ch P Hch Hstr
+           => {| er_state := on_terminal P;
+                 er_ensemble := ensemble_on_terminal P;
+                 er_related := on_terminal_correct P;
+                 er_correct := ex_intro _ ch (conj Hch Hstr);
+                 er_state_le := reflexivity _ |}
+         | ParseNonTerminal nt Hvalid p' => lift_ensemble_result (state_of_parse p')
          end.
 
     Definition state_of_parse_production'
                str pat (p : parse_of_production G str pat)
-      : T
+      : ensemble_result str (fold_production' G (lookup_state fold_grammar) pat)
       := match p with
-         | ParseProductionNil Hlen => on_nil_production
+         | ParseProductionNil Hlen
+           => {| er_state := on_nil_production;
+                 er_ensemble := ensemble_on_nil_production;
+                 er_related := on_nil_production_correct (related := related);
+                 er_correct := Hlen;
+                 er_state_le := reflexivity _ |}
          | ParseProductionCons n pat pats p' p's
-           => combine_production
+           => er_combine_production
+                n
+                str
                 (state_of_parse_item p')
                 (state_of_parse_production p's)
          end.
 
     Definition state_of_parse'
                str pats (p : parse_of G str pats)
-      : T
-      := match p with
-         | ParseHead pat pats p' => state_of_parse_production p'
-         | ParseTail pat pats p' => state_of_parse p'
+      : ensemble_result str (fold_productions' G (lookup_state fold_grammar) pats)
+      := match p in parse_of _ _ pats return ensemble_result _ (fold_productions' _ _ pats) with
+         | ParseHead pat pats p' => er_lift (state_of_parse_production p') (greatest_lower_bound_correct_l _ _)
+         | ParseTail pat pats p' => er_lift (state_of_parse p') (greatest_lower_bound_correct_r _ _)
          end.
   End step.
 
-  Fixpoint state_of_parse str pats (p : parse_of G str pats) : T
+  Fixpoint state_of_parse str pats (p : parse_of G str pats)
     := @state_of_parse' (@state_of_parse) (@state_of_parse_production) str pats p
-  with state_of_parse_production str pat (p : parse_of_production G str pat) : T
+  with state_of_parse_production str pat (p : parse_of_production G str pat)
     := @state_of_parse_production' (@state_of_parse_production) (@state_of_parse_item) str pat p
-  with state_of_parse_item str it (p : parse_of_item G str it) : T
+  with state_of_parse_item str it (p : parse_of_item G str it)
     := @state_of_parse_item' (@state_of_parse) str it p.
 
-  (*Lemma fold_nt_correct nt
-    : related (fun str => inhabited (parse_of_item G str (NonTerminal (to_nonterminal nt))))
-              (lookup_state fold_grammar nt).
+  Lemma fold_grammar_correct_item str nt
+        (p : parse_of_item G str (NonTerminal nt))
+    : exists P, P str /\ related P (lookup_state fold_grammar (of_nonterminal nt)).
   Proof.
-    unfold fold_grammar.
-    SearchAbout lookup_state
-
-  Lemma fixedpoint_lower_bound_for_reachable
-
-  Lemma fold_nt_correct'
-    : forall nt, Pnt nt (lookup_state fold_grammar nt).
-  Proof.
-    unfold fold_grammar.
-    intro.
-    apply pre_Fix_grammar_fixedpoint_correct_stronger.
-    { apply Pnt_init. }
-    { apply Pnt_bottom. }
-    { intros ?? Hinvalid Hbot Hvalid.
-      apply Pnt_glb; [ assumption | solve [ eauto ] | ].
-      unfold step_constraints, fixedpoint_from_fold.
-      unfold fold_constraints.
-      apply Pnt_lift; [ assumption | ].
-      apply fold_productions'_correct.
-      assumption. }
+    pose proof (@state_of_parse_item _ _ p) as p'.
+    unfold fold_item' in p'.
+    exists (er_ensemble p').
+    split; [ apply p' | ].
+    eapply (related_monotonic _); apply p'.
   Qed.
 
-
-  Lemma fold_production'_correct
-        f
-        (IHf : forall nt, Pnt nt (f nt))
-        pat
-  : Ppat pat (fold_production' (fun nt => f (of_nonterminal nt)) pat).
+  Lemma fold_grammar_correct str nt
+        (p : parse_of G str (Lookup G nt))
+    : exists P, P str /\ related P (lookup_state fold_grammar (of_nonterminal nt)).
   Proof.
-    unfold fold_production'.
-    induction pat; simpl.
-    { apply Ppat_nil. }
-    { edestruct (_ : item _).
-      { apply Ppat_cons_t; trivial. }
-      { apply Ppat_cons_nt; trivial. } }
+    destruct (is_valid_nonterminal initial_nonterminals_data (of_nonterminal nt)) eqn:Hvalid.
+    { apply fold_grammar_correct_item; constructor.
+      { apply initial_nonterminals_correct; assumption. }
+      { assumption. } }
+    { unfold fold_grammar.
+      rewrite (lookup_state_invalid_pre_Fix_grammar _ G) by assumption.
+      do 2 esplit; [ | eexact (bottom_related (related := related)) ].
+      constructor. }
   Qed.
-
-  Lemma fold_productions'_correct
-        f
-        (IHf : forall nt, Pnt nt (f nt))
-        pats
-  : Ppats pats (fold_productions' (fun nt => f (of_nonterminal nt)) pats).
-  Proof.
-    unfold fold_productions'.
-    induction pats as [ | x xs IHxs ]; intros.
-    { simpl; apply Ppats_nil. }
-    { simpl; apply Ppats_cons; trivial; [].
-      { apply fold_production'_correct; trivial. } }
-  Qed.
-
-  Lemma fold_nt_correct'
-    : forall nt, Pnt nt (lookup_state fold_grammar nt).
-  Proof.
-    unfold fold_grammar.
-    intro.
-    apply pre_Fix_grammar_fixedpoint_correct_stronger.
-    { apply Pnt_init. }
-    { apply Pnt_bottom. }
-    { intros ?? Hinvalid Hbot Hvalid.
-      apply Pnt_glb; [ assumption | solve [ eauto ] | ].
-      unfold step_constraints, fixedpoint_from_fold.
-      unfold fold_constraints.
-      apply Pnt_lift; [ assumption | ].
-      apply fold_productions'_correct.
-      assumption. }
-  Qed.*)
 End fold_correctness.
+
+Global Arguments fold_grammar_correct {_ HSLM HSL _ _ _ _ _} [_ _ _] _.
+Global Arguments fold_grammar_correct_item {_ HSLM HSL _ _ _ _ _} [_ _ _] _.
