src/Common/Notations.v
@@ -3,6 +3,7 @@ Reserved Infix "@" (left associativity, at level 77).
 Reserved Notation "\ x , e" (at level 78).
 Reserved Notation "\ ! , e" (at level 78).
 Reserved Infix "⊓" (at level 80).
+Reserved Infix "⊔" (at level 80).
 Reserved Infix "=s" (at level 70, no associativity).
 Reserved Infix "=b" (at level 70, no associativity).
 Reserved Notation "s ~= [ ch ]" (at level 70, no associativity).
